viper-total-heaps/DummyRel.thy
@@ -3,20 +3,6 @@ theory DummyRel
 begin
 
 
-lemma exhale_rel_star_2: "True" by (rule HOL.TrueI)
-lemma exhale_rel_imp_2: "True" by (rule HOL.TrueI)
-lemma exhale_rel_propagate_post: "True" by (rule HOL.TrueI)
-lemma exhale_rel_cond: "True" by (rule HOL.TrueI)
-lemma framing_exhI_exprs_wf_rel: "True" by (rule HOL.TrueI)
-lemma exhale_field_acc_rel_assms_perm_eval: "True" by (rule HOL.TrueI)
-lemma exhale_field_acc_rel_perm_success_def: "True" by (rule HOL.TrueI)
-lemma exhale_field_acc_rel_assms_ref_eval: "True" by (rule HOL.TrueI)
-lemma exhale_field_acc_rel_assms_def: "True" by (rule HOL.TrueI)
-lemma exhale_rel_field_acc_upd_rel: "True" by (rule HOL.TrueI)
-lemma exhale_rel_field_acc: "True" by (rule HOL.TrueI)
-lemma exhale_rel_pure: "True" by (rule HOL.TrueI)
-lemma exhale_rel_propagate_pre_no_inv_same_exh: "True" by (rule HOL.TrueI)
-lemma exhale_rel_propagate_pre_no_inv: "True" by (rule HOL.TrueI)
 lemma method_call_stmt_rel_inst: "True" by (rule HOL.TrueI)
 
 
