viper-total-heaps/StmtRelML.thy
@@ -1,5 +1,5 @@
 theory StmtRelML
-imports Boogie_Lang.HelperML ExprWfRelML StmtRel InhaleRelML ExhaleRelML ViperBoogieHelperML
+imports Boogie_Lang.HelperML ExprWfRelML StmtRel InhaleRelML ExhaleRelML PredicateRelML ViperBoogieHelperML
 begin
 
 ML \<open>
@@ -134,6 +134,9 @@ ML \<open>
   | InhaleHint of (atomic_inhale_rel_hint inhale_rel_complete_hint)
   | ExhaleHint of (atomic_exhale_rel_hint exhale_rel_complete_hint)
   | AssertHint of (atomic_exhale_rel_hint assert_rel_complete_hint)
+  | UnfoldHint of
+       atomic_exhale_rel_hint *
+       (atomic_inhale_rel_hint inhale_rel_complete_hint)
   | MethodCallHint of 
        string * (* callee name *)
        thm list * (* Boogie return variable lookup decl theorem *)
@@ -345,6 +348,8 @@ ML \<open>
         (Rmsg' "AtomicAssert Start" (resolve_tac ctxt [#assert_stmt_rel_thm assert_complete_hint]) ctxt) THEN'
         (Rmsg' "AtomicAssert Init" ((#init_tac assert_complete_hint) basic_info (#setup_well_def_state_tac assert_complete_hint basic_info) ctxt) ctxt) THEN' 
         (assert_rel_tac ctxt exhale_info assert_complete_hint)
+     | UnfoldHint (atomic_exhale_hint, inhale_hint) =>
+        (pred_unfold_tac ctxt inhale_info exhale_info basic_info atomic_exhale_hint inhale_hint)
      | MethodCallHint (callee_name, rets_lookup_decl_thms, inhale_info_call, exhale_info_call, exh_pre_complete_hint, inh_post_complete_hint) => 
         let val callee_data = Symtab.lookup (#method_data_table basic_info) callee_name |> Option.valOf in
         (Rmsg' "MethodCall Start" (resolve_tac ctxt [@{thm method_call_stmt_rel_inst} OF [#consistency_wf_thm basic_info, #consistency_down_mono_thm basic_info]]) ctxt) THEN'
